src/cddl/spec/CDDL.Spec.MapGroup.fsti
@@ -1,25 +1,26 @@
 module CDDL.Spec.MapGroup
 include CDDL.Spec.MapGroup.Base
-module Cbor = CBOR.Spec.API.Type
 module U8 = FStar.UInt8
 module U64 = FStar.UInt64
 module U = CBOR.Spec.Util
+module Map = CDDL.Spec.Map
+open CBOR.Spec.API.Type
 
 let cbor_map_disjoint_from_footprint
-  (m: Cbor.cbor_map)
+  (m: cbor_map)
   (f: typ)
 : Tot prop
-= forall x . Some? (Cbor.cbor_map_get m x) ==> ~ (f x)
+= forall x . Some? (cbor_map_get m x) ==> ~ (f x)
 
 let map_group_footprint
   (g: map_group)
   (f: typ)
 : Tot prop
-= forall m m' . (Cbor.cbor_map_disjoint m m' /\ cbor_map_disjoint_from_footprint m' f) ==>
-  begin match apply_map_group_det g m, apply_map_group_det g (m `Cbor.cbor_map_union` m') with
+= forall m m' . (cbor_map_disjoint m m' /\ cbor_map_disjoint_from_footprint m' f) ==>
+  begin match apply_map_group_det g m, apply_map_group_det g (m `cbor_map_union` m') with
   | MapGroupCutFail, MapGroupCutFail
   | MapGroupFail, MapGroupFail -> True
-  | MapGroupDet _ r, MapGroupDet _ r' -> r' == r `Cbor.cbor_map_union` m'
+  | MapGroupDet _ r, MapGroupDet _ r' -> r' == r `cbor_map_union` m'
   | _ -> False
   end
 
@@ -38,38 +39,42 @@ let map_group_footprint_equiv
 let map_group_footprint_elim
   (g: map_group)
   (f: typ)
-  (m m' : Cbor.cbor_map)
+  (m m' : cbor_map)
 : Lemma
   (requires
     map_group_footprint g f /\
-    Cbor.cbor_map_disjoint m m' /\
+    cbor_map_disjoint m m' /\
     cbor_map_disjoint_from_footprint m' f
   )
   (ensures
-  begin match apply_map_group_det g m, apply_map_group_det g (m `Cbor.cbor_map_union` m') with
+  begin match apply_map_group_det g m, apply_map_group_det g (m `cbor_map_union` m') with
   | MapGroupCutFail, MapGroupCutFail
   | MapGroupFail, MapGroupFail -> True
-  | MapGroupDet _ r, MapGroupDet _ r' -> r' == r `Cbor.cbor_map_union` m'
+  | MapGroupDet c r, MapGroupDet c' r' -> c' == c /\ r' == r `cbor_map_union` m'
   | _ -> False
   end
   )
-= ()
+= match apply_map_group_det g m, apply_map_group_det g (m `cbor_map_union` m') with
+  | MapGroupDet c r, MapGroupDet c' r' ->
+    assert (r' == r `cbor_map_union` m');
+    assert (cbor_map_equal c' c)
+  | _ -> ()
 
 #restart-solver
 let map_group_footprint_intro
   (g: map_group)
   (f: typ)
-  (prf: (m: _) -> (m' : Cbor.cbor_map) ->
+  (prf: (m: _) -> (m' : cbor_map) ->
     Lemma
     (requires
-      Cbor.cbor_map_disjoint m m' /\
+      cbor_map_disjoint m m' /\
       cbor_map_disjoint_from_footprint m' f
     )
     (ensures
-    begin match apply_map_group_det g m, apply_map_group_det g (m `Cbor.cbor_map_union` m') with
+    begin match apply_map_group_det g m, apply_map_group_det g (m `cbor_map_union` m') with
     | MapGroupCutFail, MapGroupCutFail
     | MapGroupFail, MapGroupFail -> True
-    | MapGroupDet _ r, MapGroupDet _ r' -> r' == r `Cbor.cbor_map_union` m'
+    | MapGroupDet _ r, MapGroupDet _ r' -> r' == r `cbor_map_union` m'
     | _ -> False
     end
     )
@@ -86,20 +91,20 @@ let map_group_footprint_consumed
 : Lemma
   (requires
     map_group_footprint g f /\
-    Cbor.cbor_map_disjoint m m' /\
+    cbor_map_disjoint m m' /\
     cbor_map_disjoint_from_footprint m' f /\
-    (MapGroupDet? (apply_map_group_det g m) \/ MapGroupDet? (apply_map_group_det g (m `Cbor.cbor_map_union` m')))
+    (MapGroupDet? (apply_map_group_det g m) \/ MapGroupDet? (apply_map_group_det g (m `cbor_map_union` m')))
   )
   (ensures (
-    match apply_map_group_det g m, apply_map_group_det g (m `Cbor.cbor_map_union` m') with
+    match apply_map_group_det g m, apply_map_group_det g (m `cbor_map_union` m') with
     | MapGroupDet c _, MapGroupDet c' _ -> c == c'
     | _ -> False
   ))
-  [SMTPat (map_group_footprint g f); SMTPat (apply_map_group_det g (m `Cbor.cbor_map_union` m'))]
+  [SMTPat (map_group_footprint g f); SMTPat (apply_map_group_det g (m `cbor_map_union` m'))]
 = let MapGroupDet c r = apply_map_group_det g m in
-  let MapGroupDet c' r' = apply_map_group_det g (m `Cbor.cbor_map_union` m') in
-  Cbor.cbor_map_union_assoc c r m';
-  Cbor.cbor_map_disjoint_union_simpl_r c c' r'
+  let MapGroupDet c' r' = apply_map_group_det g (m `cbor_map_union` m') in
+  cbor_map_union_assoc c r m';
+  cbor_map_disjoint_union_simpl_r c c' r'
 
 #restart-solver
 let map_group_footprint_is_consumed
@@ -111,13 +116,13 @@ let map_group_footprint_is_consumed
     map_group_footprint g f
   )
   (ensures (
-    match apply_map_group_det g m, apply_map_group_det g (Cbor.cbor_map_filter (matches_map_group_entry f any) m) with
+    match apply_map_group_det g m, apply_map_group_det g (cbor_map_filter (matches_map_group_entry f any) m) with
     | MapGroupDet _ _, MapGroupDet _ _
     | MapGroupFail, MapGroupFail
     | MapGroupCutFail, MapGroupCutFail -> True
     | _ -> False
   ))
-= Cbor.cbor_map_split (matches_map_group_entry f any) m
+= cbor_map_split (matches_map_group_entry f any) m
 
 let map_group_footprint_consumed_disjoint
   (g: map_group)
@@ -135,8 +140,8 @@ let map_group_footprint_consumed_disjoint
       cbor_map_disjoint_from_footprint c f'
     | _ -> False
   ))
-= Cbor.cbor_map_split (matches_map_group_entry f any) m;
-  map_group_footprint_consumed g f (Cbor.cbor_map_filter (matches_map_group_entry f any) m) (Cbor.cbor_map_filter (U.notp (matches_map_group_entry f any)) m)
+= cbor_map_split (matches_map_group_entry f any) m;
+  map_group_footprint_consumed g f (cbor_map_filter (matches_map_group_entry f any) m) (cbor_map_filter (U.notp (matches_map_group_entry f any)) m)
 
 #restart-solver
 let map_group_footprint_concat
@@ -183,55 +188,55 @@ let map_group_footprint_zero_or_one
 let map_group_footprint_consumes_all
   (g1: map_group)
   (f1: typ)
-  (m1: Cbor.cbor_map)
+  (m1: cbor_map)
 : Lemma
   (requires (
     map_group_footprint g1 f1 /\
-    apply_map_group_det g1 m1 == MapGroupDet m1 Cbor.cbor_map_empty
+    apply_map_group_det g1 m1 == MapGroupDet m1 cbor_map_empty
   ))
   (ensures (
-    Cbor.cbor_map_filter (matches_map_group_entry f1 any) m1 == m1 /\
-    Cbor.cbor_map_filter (U.notp (matches_map_group_entry f1 any)) m1 == Cbor.cbor_map_empty
+    cbor_map_filter (matches_map_group_entry f1 any) m1 == m1 /\
+    cbor_map_filter (U.notp (matches_map_group_entry f1 any)) m1 == cbor_map_empty
   ))
 = let phi1 = matches_map_group_entry f1 any in
-  Cbor.cbor_map_split phi1 m1;
-  map_group_footprint_elim g1 f1 (Cbor.cbor_map_filter phi1 m1) (Cbor.cbor_map_filter (U.notp phi1) m1); 
-  map_group_footprint_consumed g1 f1 (Cbor.cbor_map_filter phi1 m1) (Cbor.cbor_map_filter (U.notp phi1) m1);
-  let MapGroupDet c1 r1 = apply_map_group_det g1 (Cbor.cbor_map_filter phi1 m1) in
-  let MapGroupDet c' r' = apply_map_group_det g1 (Cbor.cbor_map_filter phi1 m1 `Cbor.cbor_map_union` Cbor.cbor_map_filter (U.notp phi1) m1) in
-  assert (Cbor.cbor_map_empty == r1 `Cbor.cbor_map_union` Cbor.cbor_map_filter (U.notp phi1) m1);
-  Cbor.cbor_map_ext Cbor.cbor_map_empty (Cbor.cbor_map_filter (U.notp phi1) m1);
+  cbor_map_split phi1 m1;
+  map_group_footprint_elim g1 f1 (cbor_map_filter phi1 m1) (cbor_map_filter (U.notp phi1) m1); 
+  map_group_footprint_consumed g1 f1 (cbor_map_filter phi1 m1) (cbor_map_filter (U.notp phi1) m1);
+  let MapGroupDet c1 r1 = apply_map_group_det g1 (cbor_map_filter phi1 m1) in
+  let MapGroupDet c' r' = apply_map_group_det g1 (cbor_map_filter phi1 m1 `cbor_map_union` cbor_map_filter (U.notp phi1) m1) in
+  assert (cbor_map_empty == r1 `cbor_map_union` cbor_map_filter (U.notp phi1) m1);
+  cbor_map_ext cbor_map_empty (cbor_map_filter (U.notp phi1) m1);
   ()
 
 #restart-solver
 let map_group_footprint_concat_consumes_all
   (g1 g2: map_group)
   (f1 f2: typ)
-  (m1 m2: Cbor.cbor_map)
+  (m1 m2: cbor_map)
 : Lemma
   (requires (
     map_group_footprint g1 f1 /\
     map_group_footprint g2 f2 /\
-    apply_map_group_det g1 m1 == MapGroupDet m1 Cbor.cbor_map_empty /\
-    apply_map_group_det g2 m2 == MapGroupDet m2 Cbor.cbor_map_empty /\
+    apply_map_group_det g1 m1 == MapGroupDet m1 cbor_map_empty /\
+    apply_map_group_det g2 m2 == MapGroupDet m2 cbor_map_empty /\
     typ_disjoint f1 f2
   ))
   (ensures (
-    m1 `Cbor.cbor_map_disjoint` m2 /\
-    apply_map_group_det (g1 `map_group_concat` g2) (m1 `Cbor.cbor_map_union` m2) == MapGroupDet (m1 `Cbor.cbor_map_union` m2) Cbor.cbor_map_empty
+    m1 `cbor_map_disjoint` m2 /\
+    apply_map_group_det (g1 `map_group_concat` g2) (m1 `cbor_map_union` m2) == MapGroupDet (m1 `cbor_map_union` m2) cbor_map_empty
   ))
 = map_group_footprint_consumes_all g1 f1 m1;
   map_group_footprint_consumes_all g2 f2 m2;
-  let x = apply_map_group_det (g1 `map_group_concat` g2) (m1 `Cbor.cbor_map_union` m2) in
+  let x = apply_map_group_det (g1 `map_group_concat` g2) (m1 `cbor_map_union` m2) in
   assert (MapGroupDet? x);
-  assert (MapGroupDet?.consumed x `Cbor.cbor_map_equal` (m1 `Cbor.cbor_map_union` m2));
-  assert (MapGroupDet?.remaining x `Cbor.cbor_map_equal` Cbor.cbor_map_empty);
+  assert (MapGroupDet?.consumed x `cbor_map_equal` (m1 `cbor_map_union` m2));
+  assert (MapGroupDet?.remaining x `cbor_map_equal` cbor_map_empty);
   ()
 
 #restart-solver
 let map_group_footprint_match_item_for
   (cut: bool)
-  (key: Cbor.cbor)
+  (key: cbor)
   (value: typ)
 : Lemma
   (ensures (
@@ -243,10 +248,10 @@ let map_group_footprint_match_item_for
     g
     (t_literal key)
     (fun m m' ->
-       assert (None? (Cbor.cbor_map_get m' key));
-       match apply_map_group_det g m, apply_map_group_det g (m `Cbor.cbor_map_union` m') with
+       assert (None? (cbor_map_get m' key));
+       match apply_map_group_det g m, apply_map_group_det g (m `cbor_map_union` m') with
        | MapGroupDet _ r, MapGroupDet _ r' ->
-         Cbor.cbor_map_ext r' (r `Cbor.cbor_map_union` m')
+         cbor_map_ext r' (r `cbor_map_union` m')
        | _ -> ()
     )
 
@@ -256,7 +261,7 @@ let map_group_footprint_filter
   (f: typ)
 : Lemma
   (requires
-    forall (x: (Cbor.cbor & Cbor.cbor)) . U.notp phi x ==> f (fst x)
+    forall (x: (cbor & cbor)) . U.notp phi x ==> f (fst x)
   )
   (ensures (
     map_group_footprint (map_group_filter phi) f
@@ -268,10 +273,10 @@ let map_group_footprint_filter
     f
     (fun m m' ->
       let MapGroupDet _ r = apply_map_group_det g m in
-      let MapGroupDet _ r' = apply_map_group_det g (m `Cbor.cbor_map_union` m') in
-      Cbor.cbor_map_disjoint_union_filter phi m m';
-      Cbor.cbor_map_filter_for_all phi m';
-      assert (r' == r `Cbor.cbor_map_union` m')
+      let MapGroupDet _ r' = apply_map_group_det g (m `cbor_map_union` m') in
+      cbor_map_disjoint_union_filter phi m m';
+      cbor_map_filter_for_all phi m';
+      assert (r' == r `cbor_map_union` m')
     )
 
 let map_group_footprint_zero_or_more_match_item
@@ -281,8 +286,8 @@ let map_group_footprint_zero_or_more_match_item
   [SMTPat (map_group_footprint (map_group_zero_or_more (map_group_match_item false key value)))]
 = ()
 
-let cbor_map_included (c' c : Cbor.cbor_map) : Tot prop =
-  (forall x . Some? (Cbor.cbor_map_get c' x) ==> Cbor.cbor_map_get c' x == Cbor.cbor_map_get c x)
+let cbor_map_included (c' c : cbor_map) : Tot prop =
+  (forall x . Some? (cbor_map_get c' x) ==> cbor_map_get c' x == cbor_map_get c x)
 
 let restrict_map_group
   (g g': map_group)
@@ -318,14 +323,14 @@ let restrict_map_group_refl
 
 let restrict_map_group_match_item_for
   (cut: bool)
-  (key: Cbor.cbor)
+  (key: cbor)
   (value: typ)
 : Lemma
   (restrict_map_group (map_group_match_item_for cut key value) (map_group_match_item_for cut key value))
 = ()
 
 let restrict_map_group_filter
-  (f: (Cbor.cbor & Cbor.cbor) -> Tot bool)
+  (f: (cbor & cbor) -> Tot bool)
 : Lemma
   (restrict_map_group (map_group_filter f) map_group_nop)
   [SMTPat (restrict_map_group (map_group_filter f) map_group_nop)]
@@ -408,7 +413,7 @@ let map_group_choice_compatible
   (left right: map_group)
 : Tot prop
 = forall x . match apply_map_group_det right x with
-  | MapGroupDet _ rem -> rem == Cbor.cbor_map_empty ==> MapGroupFail? (apply_map_group_det left x)
+  | MapGroupDet _ rem -> rem == cbor_map_empty ==> MapGroupFail? (apply_map_group_det left x)
   | _ -> True
 
 #restart-solver
@@ -416,7 +421,7 @@ let map_group_choice_compatible_intro
   (left right: map_group)
   (prf: (x: _) -> Lemma
     (requires begin match apply_map_group_det right x with
-     | MapGroupDet _ rem -> rem == Cbor.cbor_map_empty
+     | MapGroupDet _ rem -> rem == cbor_map_empty
      | _ -> False
     end)
     (ensures MapGroupFail? (apply_map_group_det left x))
@@ -428,7 +433,7 @@ let map_group_choice_compatible_intro
 #restart-solver
 val map_group_choice_compatible_match_item_for
   (cut: bool)
-  (key: Cbor.cbor)
+  (key: cbor)
   (value: typ)
   (right: map_group)
   (fp: typ)
@@ -445,7 +450,7 @@ let map_group_choice_compatible_no_cut
   (left right: map_group)
 : Tot prop
 = forall x . match apply_map_group_det right x with
-  | MapGroupDet _ rem -> rem == Cbor.cbor_map_empty ==> ~ (MapGroupCutFail? (apply_map_group_det left x))
+  | MapGroupDet _ rem -> rem == cbor_map_empty ==> ~ (MapGroupCutFail? (apply_map_group_det left x))
   | _ -> True
 
 let map_group_choice_compatible_implies_no_cut
@@ -460,7 +465,7 @@ let map_group_fail_concat_intro
   (f1: typ)
   (g2: det_map_group)
   (f2: typ)
-  (x: Cbor.cbor_map)
+  (x: cbor_map)
 : Lemma
   (requires (
     map_group_footprint g1 f1 /\
@@ -478,15 +483,15 @@ let map_group_fail_concat_intro
   else begin
     let MapGroupDet c1 r1 = apply_map_group_det g1 x in
     map_group_footprint_consumed_disjoint g1 f1 f2 x;
-    Cbor.cbor_map_disjoint_union_comm c1 r1
+    cbor_map_disjoint_union_comm c1 r1
   end
 
 let map_group_consumes_all
   (g: map_group)
-  (x: Cbor.cbor_map)
+  (x: cbor_map)
 : Tot prop
 = match apply_map_group_det g x with
-  | MapGroupDet _ r -> r == Cbor.cbor_map_empty
+  | MapGroupDet _ r -> r == cbor_map_empty
   | _ -> False
 
 let map_group_choice_compatible_concat_left
@@ -516,7 +521,7 @@ let map_group_concat_no_cut_intro
   (f1: typ)
   (g2: det_map_group)
   (f2: typ)
-  (x: Cbor.cbor_map)
+  (x: cbor_map)
 : Lemma
   (requires (
     map_group_footprint g1 f1 /\
@@ -533,7 +538,7 @@ let map_group_concat_no_cut_intro
   else begin
     let MapGroupDet c1 r1 = apply_map_group_det g1 x in
     map_group_footprint_consumed_disjoint g1 f1 f2 x;
-    Cbor.cbor_map_disjoint_union_comm c1 r1
+    cbor_map_disjoint_union_comm c1 r1
   end
 
 #restart-solver
@@ -630,7 +635,7 @@ let map_group_choice_compatible_no_cut_choice_right
 = ()
 
 let map_group_choice_compatible_no_cut_match_item_for_no_cut
-  (key: Cbor.cbor)
+  (key: cbor)
   (value: typ)
   (g: det_map_group)
 : Lemma
@@ -646,7 +651,7 @@ let map_group_choice_compatible_no_cut_zero_or_more_match_item_left
 = ()
 
 let map_group_choice_compatible_no_cut_match_item_for_cut
-  (key: Cbor.cbor)
+  (key: cbor)
   (value: typ)
   (g: det_map_group)
   (f: typ)
@@ -663,8 +668,8 @@ let map_group_choice_compatible_no_cut_match_item_for_cut
 val map_group_footprint_concat_consumes_all_recip
   (g1 g2: map_group)
   (f1 f2: typ)
-  (m: Cbor.cbor_map)
-: Pure (Cbor.cbor_map & Cbor.cbor_map)
+  (m: cbor_map)
+: Pure (cbor_map & cbor_map)
   (requires (
     map_group_footprint g1 f1 /\
     map_group_footprint g2 f2 /\
@@ -672,17 +677,17 @@ val map_group_footprint_concat_consumes_all_recip
     map_group_consumes_all (g1 `map_group_concat` g2) m
   ))
   (ensures (fun (m1, m2) ->
-    m1 `Cbor.cbor_map_disjoint` m2 /\
-    apply_map_group_det g1 m1 == MapGroupDet m1 Cbor.cbor_map_empty /\
-    apply_map_group_det g2 m2 == MapGroupDet m2 Cbor.cbor_map_empty /\
-    m1 `Cbor.cbor_map_union` m2 == m
+    m1 `cbor_map_disjoint` m2 /\
+    apply_map_group_det g1 m1 == MapGroupDet m1 cbor_map_empty /\
+    apply_map_group_det g2 m2 == MapGroupDet m2 cbor_map_empty /\
+    m1 `cbor_map_union` m2 == m
   ))
 
 #restart-solver
 let map_group_footprint_concat_consumes_all_recip'
   (g1 g2: map_group)
   (f1 f2: typ)
-  (m: Cbor.cbor_map)
+  (m: cbor_map)
 : Lemma
   (requires (
     map_group_footprint g1 f1 /\
@@ -692,17 +697,17 @@ let map_group_footprint_concat_consumes_all_recip'
   ))
   (ensures exists m1m2 .
     (let (m1, m2) = m1m2 in
-    m1 `Cbor.cbor_map_disjoint` m2 /\
-    apply_map_group_det g1 m1 == MapGroupDet m1 Cbor.cbor_map_empty /\
-    apply_map_group_det g2 m2 == MapGroupDet m2 Cbor.cbor_map_empty /\
-    m1 `Cbor.cbor_map_union` m2 == m
+    m1 `cbor_map_disjoint` m2 /\
+    apply_map_group_det g1 m1 == MapGroupDet m1 cbor_map_empty /\
+    apply_map_group_det g2 m2 == MapGroupDet m2 cbor_map_empty /\
+    m1 `cbor_map_union` m2 == m
   ))
 = let (_, _) = map_group_footprint_concat_consumes_all_recip g1 g2 f1 f2 m in
   ()
 
 #restart-solver
 let map_group_choice_compatible_match_item_for_concat_right
-  (k: Cbor.cbor)
+  (k: cbor)
   (v: typ)
   (g1 g2: det_map_group)
   (f1 f2: typ)
@@ -722,7 +727,7 @@ let map_group_choice_compatible_match_item_for_concat_right
 #restart-solver
 let map_group_choice_compatible_match_item_for_zero_or_one_right
   (cut: bool)
-  (k: Cbor.cbor)
+  (k: cbor)
   (v: typ)
   (g: det_map_group)
 : Lemma
@@ -736,7 +741,7 @@ let map_group_choice_compatible_match_item_for_zero_or_one_right
 
 #restart-solver
 let map_group_choice_compatible_match_item_for_same
-  (k: Cbor.cbor)
+  (k: cbor)
   (v1 v2: typ)
   (cut2: bool)
 : Lemma
@@ -749,38 +754,35 @@ let map_group_choice_compatible_match_item_for_same
 = ()
 
 let cbor_map_in_footprint
-  (m: Cbor.cbor_map)
+  (m: cbor_map)
   (f: typ)
 : Tot prop
-= forall x . Some? (Cbor.cbor_map_get m x) ==> (f x)
+= forall x . Some? (cbor_map_get m x) ==> (f x)
 
-(* // TODO: use a map rather than a list
 unfold
 let map_group_parser_spec_arg_common
   (source: det_map_group)
   (source_fp: typ)
-  (x: list (Cbor.raw_data_item & Cbor.raw_data_item)) // list needed because I need to preserve the order of elements when parsing a table
+  (m: cbor_map)
 : Tot prop
 = 
-    let m = Cbor.cbor_map_of_list x in
-    List.Tot.no_repeats_p (List.Tot.map fst x) /\
     map_group_footprint source source_fp /\
-    Cbor.cbor_map_in_footprint m source_fp
+    cbor_map_in_footprint m source_fp
 
 unfold
 let map_group_parser_spec_arg_prop
   (source: det_map_group)
   (source_fp: typ)
-  (x: list (Cbor.raw_data_item & Cbor.raw_data_item)) // list needed because I need to preserve the order of elements when parsing a table
+  (x: cbor_map)
 : Tot prop
 = map_group_parser_spec_arg_common source source_fp x /\
-  MapGroupDet? (apply_map_group_det source (Cbor.cbor_map_of_list x))
+  MapGroupDet? (apply_map_group_det source x)
 
 let map_group_parser_spec_arg
   (source: det_map_group)
   (source_fp: typ)
 : Tot Type0
-= (x: list (Cbor.raw_data_item & Cbor.raw_data_item) {
+= (x: cbor_map {
     map_group_parser_spec_arg_prop source source_fp x
   })
 
@@ -788,12 +790,12 @@ let map_group_parser_spec_ret
   (source: det_map_group)
   (source_fp: typ)
   (#target: Type0)
-  (target_size: target -> GTot nat)
-  (target_prop: target -> prop)
+  (target_size: target -> Tot nat)
+  (target_prop: target -> bool)
   (x: map_group_parser_spec_arg source source_fp)
 : Tot Type0
 = (y: target { 
-    target_size y <= List.Tot.length x // not everything is parsed, especially for choice
+    target_size y <= cbor_map_length x // not everything is parsed, especially for choice
     /\ target_prop y
   })
 
@@ -801,116 +803,115 @@ let map_group_parser_spec
   (source: det_map_group)
   (source_fp: typ)
   (#target: Type0)
-  (target_size: target -> GTot nat)
-  (target_prop: target -> prop)
+  (target_size: target -> Tot nat)
+  (target_prop: target -> bool)
 : Type0
-= (x: map_group_parser_spec_arg source source_fp) -> GTot (map_group_parser_spec_ret source source_fp target_size target_prop x)
+= (x: map_group_parser_spec_arg source source_fp) -> Tot (map_group_parser_spec_ret source source_fp target_size target_prop x)
 
 unfold
 let map_group_serializer_spec_arg_prop
   (source: det_map_group)
   (source_fp: typ)
-  (x: list (Cbor.raw_data_item & Cbor.raw_data_item)) // list needed because I need to preserve the order of elements when parsing a table
+  (x: cbor_map)
 : Tot prop
 = map_group_parser_spec_arg_common source source_fp x /\
-  begin match apply_map_group_det source (Cbor.cbor_map_of_list x) with
-  | MapGroupDet _ res -> res == Cbor.cbor_map_empty // everything is consumed
+  begin match apply_map_group_det source x with
+  | MapGroupDet _ res -> res `cbor_map_equal` cbor_map_empty // everything is consumed
   | _ -> False
   end
+
+let map_group_serializer_spec_ret
+  (#source: det_map_group)
+  (#source_fp: typ)
+  (#target: Type0)
+  (#target_size: target -> Tot nat)
+  (#target_prop: target -> bool)
+  (p: map_group_parser_spec source source_fp target_size target_prop)
+  (x: target { target_prop x })
+: Tot Type
+= (y: cbor_map {
+    map_group_serializer_spec_arg_prop source source_fp y /\
+    target_size x == cbor_map_length y /\
+    p y == x
+  })
+
+let map_group_serializer_spec_ret_intro
+  (#source: det_map_group)
+  (#source_fp: typ)
+  (#target: Type0)
+  (#target_size: target -> Tot nat)
+  (#target_prop: target -> bool)
+  (p: map_group_parser_spec source source_fp target_size target_prop)
+  (x: target { target_prop x })
+  (y: cbor_map)
+  (sq1: squash (map_group_serializer_spec_arg_prop source source_fp y))
+  (sq2: squash (target_size x == cbor_map_length y))
+  (sq3: squash (p y == x))
+: Tot (map_group_serializer_spec_ret p x)
+= y
 
 #restart-solver
 let map_group_serializer_spec
   (#source: det_map_group)
   (#source_fp: typ)
   (#target: Type0)
-  (#target_size: target -> GTot nat)
-  (#target_prop: target -> prop)
+  (#target_size: target -> Tot nat)
+  (#target_prop: target -> bool)
   (p: map_group_parser_spec source source_fp target_size target_prop)
 : Type0
-= (x: target { target_prop x }) -> GTot (y: list _ {
-    map_group_serializer_spec_arg_prop source source_fp y /\
-    target_size x == List.Tot.length y /\
-    p y == x
-  })
+= (x: target { target_prop x }) -> Tot (map_group_serializer_spec_ret p x)
 
-[@@erasable]
 noeq
 type mg_spec
   (source: det_map_group)
   (source_fp: typ)
   (target: Type0)
+  (inj: bool)
 : Type
 = {
-  mg_size: target -> GTot nat;
-  mg_serializable: target -> prop;
+  mg_size: target -> Tot nat;
+  mg_serializable: target -> bool;
   mg_parser: map_group_parser_spec source source_fp mg_size mg_serializable;
   mg_serializer: map_group_serializer_spec mg_parser;
+  mg_inj: squash (inj ==> (forall (c: cbor_map { map_group_serializer_spec_arg_prop source source_fp c }) . mg_serializer (mg_parser c) == c));
 }
 
-let mg_spec_coerce_target_prop
+let mg_spec_ext
   (#source: det_map_group)
-  (#source_fp: typ)
+  (#source_fp1: typ)
   (#target: Type0)
-  (p: mg_spec source source_fp target)
-  (target_size': target -> GTot nat {
+  (#inj: bool)
+  (p: mg_spec source source_fp1 target inj)
+  (source_fp2: typ {
+    typ_equiv source_fp1 source_fp2
+  })
+  (target_size': target -> Tot nat {
     forall x . target_size' x == p.mg_size x
   })
-  (target_prop': target -> prop {
+  (target_prop': target -> bool {
     forall x . target_prop' x <==> p.mg_serializable x
   })
-: mg_spec source source_fp target
+: mg_spec source source_fp2 target inj
 = {
   mg_size = target_size';
   mg_serializable = target_prop';
-  mg_parser = (p.mg_parser <: map_group_parser_spec source source_fp target_size' target_prop');
+  mg_parser = (p.mg_parser <: map_group_parser_spec source source_fp2 target_size' target_prop');
   mg_serializer = p.mg_serializer;
+  mg_inj = ();
 }
-
-let rec list_forall_memP_filter
-  (#t: Type)
-  (f: t -> bool)
-  (l: list t)
-: Lemma
-  (requires (forall x . List.Tot.memP x l ==> f x))
-  (ensures (List.Tot.filter f l == l))
-= match l with
-  | [] -> ()
-  | _ :: q -> list_forall_memP_filter f q
-
-let rec list_filter_append
-  (#t: Type)
-  (f: t -> bool)
-  (l1 l2: list t)
-: Lemma
-  (ensures List.Tot.filter f (l1 `List.Tot.append` l2) == List.Tot.filter f l1 `List.Tot.append` List.Tot.filter f l2)
-  (decreases l1)
-= match l1 with
-  | [] -> ()
-  | _ :: q -> list_filter_append f q l2
-
-let rec list_filter_for_none
-  (#t: Type)
-  (f: t -> bool)
-  (l: list t)
-: Lemma
-  (requires (forall x . List.Tot.memP x l ==> ~ (f x)))
-  (ensures List.Tot.filter f l == [])
-= match l with
-  | [] -> ()
-  | _ :: q -> list_filter_for_none f q
 
 val parser_spec_map_group
   (source0: det_map_group)
   (#source: det_map_group)
   (#source_fp: typ)
   (#target: Type0)
-  (#target_size: target -> GTot nat)
-  (#target_prop: target -> prop)
+  (#target_size: target -> Tot nat)
+  (#target_prop: target -> bool)
   (p: map_group_parser_spec source source_fp target_size target_prop {
     restrict_map_group source0 source /\
     map_group_footprint source source_fp
   })
-  (target_prop' : target -> prop {
+  (target_prop' : target -> bool {
     forall x . target_prop' x <==> (target_prop x /\ target_size x < pow2 64)
   })
 : Tot (parser_spec (t_map source0) target target_prop')
@@ -920,24 +921,23 @@ val parser_spec_map_group_eq
   (#source: det_map_group)
   (#source_fp: typ)
   (#target: Type0)
-  (#target_size: target -> GTot nat)
-  (#target_prop: target -> prop)
+  (#target_size: target -> Tot nat)
+  (#target_prop: target -> bool)
   (p: map_group_parser_spec source source_fp target_size target_prop {
     restrict_map_group source0 source /\
     map_group_footprint source source_fp
   })
-  (target_prop' : target -> prop {
+  (target_prop' : target -> bool {
     forall x . target_prop' x <==> (target_prop x /\ target_size x < pow2 64)
   })
-  (x: CBOR.Spec.raw_data_item { t_map source0 x })
+  (w: cbor { t_map source0 w })
 : Lemma
-  (exists (f: (Cbor.raw_data_item & Cbor.raw_data_item) -> bool) .
-    (forall x . Ghost.reveal f x == matches_map_group_entry source_fp any x) /\
-    (let x' = List.Tot.filter f (Cbor.Map?.v x) in
+  (let x = CMap?.c (unpack w) in
+    (let x' = cbor_map_filter (matches_map_group_entry source_fp any) x in
     map_group_parser_spec_arg_prop source source_fp x' /\
-    parser_spec_map_group source0 p target_prop' x == p x'
+    parser_spec_map_group source0 p target_prop' w == p x'
   ))
-  [SMTPat (parser_spec_map_group source0 p target_prop' x)]
+  [SMTPat (parser_spec_map_group source0 p target_prop' w)]
 
 #restart-solver
 let serializer_spec_map_group
@@ -945,24 +945,25 @@ let serializer_spec_map_group
   (#source: det_map_group)
   (#source_fp: typ)
   (#target: Type0)
-  (#target_size: target -> GTot nat)
-  (#target_prop: target -> prop)
+  (#target_size: target -> Tot nat)
+  (#target_prop: target -> bool)
   (#p: map_group_parser_spec source source_fp target_size target_prop)
   (s: map_group_serializer_spec p {
     restrict_map_group source0 source /\
     map_group_footprint source source_fp
   })
-  (target_prop' : target -> prop {
+  (target_prop' : target -> bool {
     forall x . target_prop' x <==> (target_prop x /\ target_size x < pow2 64)
   })
 : Tot (serializer_spec (parser_spec_map_group source0 p target_prop'))
 = fun z ->
   let l = s z in
-  let MapGroupDet _ rem = apply_map_group_det source0 (Cbor.cbor_map_of_list l) in
-  Cbor.cbor_map_equiv rem Cbor.cbor_map_empty;
-  let res = Cbor.Map l in
+  let MapGroupDet _ rem = apply_map_group_det source0 l in
+  cbor_map_equiv rem cbor_map_empty;
+  let res = pack (CMap l) in
   assert (t_map source0 res);
-  Classical.forall_intro (fun f -> Classical.move_requires (list_forall_memP_filter #(Cbor.raw_data_item & Cbor.raw_data_item) f) l);
+  parser_spec_map_group_eq source0 p target_prop' res;
+  assert (cbor_map_equal (cbor_map_filter (matches_map_group_entry source_fp any) l) l);
   assert (parser_spec_map_group source0 p target_prop' res == z);
   res
 
@@ -970,38 +971,76 @@ let spec_map_group_serializable
   (#source: det_map_group)
   (#source_fp: typ)
   (#target: Type0)
-  (p: mg_spec source source_fp target)
+  (#inj: bool)
+  (p: mg_spec source source_fp target inj)
   (x: target)
-: Tot prop
-= p.mg_serializable x /\
+: Tot bool
+= p.mg_serializable x &&
   p.mg_size x < pow2 64
 
-let spec_map_group
+let spec_map_group_restrict
   (source0: det_map_group)
   (#source: det_map_group)
   (#source_fp: typ)
   (#target: Type0)
-  (p: mg_spec source source_fp target {
+  (#inj: bool)
+  (p: mg_spec source source_fp target inj {
     restrict_map_group source0 source /\
     map_group_footprint source source_fp
   })
-: Tot (spec (t_map source0) target)
+: Tot (spec (t_map source0) target false)
 = {
   serializable = spec_map_group_serializable p;
   parser = parser_spec_map_group source0 p.mg_parser _;
   serializer = serializer_spec_map_group source0 p.mg_serializer _;
+  parser_inj = ();
+}
+
+let spec_map_group_inj
+  (#source: det_map_group)
+  (#source_fp: typ)
+  (#target: Type0)
+  (#inj: bool)
+  (p: mg_spec source source_fp target inj {
+    map_group_footprint source source_fp
+  })
+  (c: cbor { t_map source c })
+: Lemma
+  (requires inj)
+  (ensures serializer_spec_map_group source p.mg_serializer (spec_map_group_serializable p) (parser_spec_map_group source p.mg_parser (spec_map_group_serializable p) c) == c)
+= let CMap l = unpack c in
+  let f = matches_map_group_entry source_fp any in
+  cbor_map_split f l;
+  let l' = cbor_map_filter f l in
+  map_group_footprint_elim source source_fp l' (cbor_map_filter (U.notp f) l);
+  assert (cbor_map_equal l' l)
+
+let spec_map_group
+  (#source: det_map_group)
+  (#source_fp: typ)
+  (#target: Type0)
+  (#inj: bool)
+  (p: mg_spec source source_fp target inj {
+    map_group_footprint source source_fp
+  })
+: Tot (spec (t_map source) target inj)
+= {
+  serializable = spec_map_group_serializable p;
+  parser = parser_spec_map_group source p.mg_parser _;
+  serializer = serializer_spec_map_group source p.mg_serializer _;
+  parser_inj = Classical.forall_intro (Classical.move_requires (spec_map_group_inj p));
 }
 
 let map_group_parser_spec_bij
   (#source: det_map_group)
   (#source_fp: typ)
   (#target1: Type0)
-  (#target_size1: target1 -> GTot nat)
-  (#target_prop1: target1 -> prop)
+  (#target_size1: target1 -> Tot nat)
+  (#target_prop1: target1 -> bool)
   (f: map_group_parser_spec source source_fp target_size1 target_prop1)
   (#target2: Type0)
-  (target_size2: target2 -> GTot nat)
-  (target_prop2: target2 -> prop)
+  (target_size2: target2 -> Tot nat)
+  (target_prop2: target2 -> bool)
   (bij: bijection target1 target2 {
     (forall x2 . target_size2 x2 == target_size1 (bij.bij_to_from x2)) /\
     (forall x2 . target_prop2 x2 <==> target_prop1 (bij.bij_to_from x2))
@@ -1013,13 +1052,13 @@ let map_group_serializer_spec_bij
   (#source: det_map_group)
   (#source_fp: typ)
   (#target1: Type0)
-  (#target_size1: target1 -> GTot nat)
-  (#target_prop1: target1 -> prop)
+  (#target_size1: target1 -> Tot nat)
+  (#target_prop1: target1 -> bool)
   (#f: map_group_parser_spec source source_fp target_size1 target_prop1)
   (s: map_group_serializer_spec f)
   (#target2: Type0)
-  (target_size2: target2 -> GTot nat)
-  (target_prop2: target2 -> prop)
+  (target_size2: target2 -> Tot nat)
+  (target_prop2: target2 -> bool)
   (bij: bijection target1 target2 {
     (forall x2 . target_size2 x2 == target_size1 (bij.bij_to_from x2)) /\
     (forall x2 . target_prop2 x2 <==> target_prop1 (bij.bij_to_from x2))
@@ -1031,118 +1070,179 @@ let mg_spec_bij_size
   (#source: det_map_group)
   (#source_fp: typ)
   (#target1: Type0)
-  (f: mg_spec source source_fp target1)
+  (#inj: bool)
+  (f: mg_spec source source_fp target1 inj)
   (#target2: Type0)
   (bij: bijection target1 target2)
   (x: target2)
-: GTot nat
+: Tot nat
 = f.mg_size (bij.bij_to_from x)
 
 let mg_spec_bij_serializable
   (#source: det_map_group)
   (#source_fp: typ)
   (#target1: Type0)
-  (f: mg_spec source source_fp target1)
+  (#inj: bool)
+  (f: mg_spec source source_fp target1 inj)
   (#target2: Type0)
   (bij: bijection target1 target2)
   (x: target2)
-: Tot prop
+: Tot bool
 = f.mg_serializable (bij.bij_to_from x)
 
 let mg_spec_bij
   (#source: det_map_group)
   (#source_fp: typ)
   (#target1: Type0)
-  (f: mg_spec source source_fp target1)
+  (#inj: bool)
+  (f: mg_spec source source_fp target1 inj)
   (#target2: Type0)
   (bij: bijection target1 target2)
-: Tot (mg_spec source source_fp target2)
+: Tot (mg_spec source source_fp target2 inj)
 = {
   mg_size = mg_spec_bij_size f bij;
   mg_serializable = mg_spec_bij_serializable f bij;
   mg_parser = map_group_parser_spec_bij f.mg_parser _ _ bij;
   mg_serializer = map_group_serializer_spec_bij f.mg_serializer _ _ bij;
+  mg_inj = ();
+}
+
+let map_group_parser_spec_nop
+  (target_size: unit -> Tot nat {
+    forall x . target_size x == 0
+  })
+  (target_prop: unit -> bool {
+    forall x . target_prop x
+  })
+: map_group_parser_spec map_group_nop t_always_false target_size target_prop
+= fun x -> ()
+
+let map_group_serializer_spec_nop
+  (target_size: unit -> Tot nat {
+    forall x . target_size x == 0
+  })
+  (target_prop: unit -> bool {
+    forall x . target_prop x
+  })
+: map_group_serializer_spec (map_group_parser_spec_nop target_size target_prop)
+= fun _ -> cbor_map_empty
+
+let mg_spec_size_nop () : Tot nat = 0
+
+let mg_spec_serializable_nop () : Tot bool = true
+
+let mg_spec_nop :
+  mg_spec map_group_nop t_always_false unit true
+= {
+  mg_size = mg_spec_size_nop;
+  mg_serializable = mg_spec_serializable_nop;
+  mg_parser = map_group_parser_spec_nop _ _;
+  mg_serializer = map_group_serializer_spec_nop _ _;
+  mg_inj = ()
 }
 
 let map_group_parser_spec_match_item_for
   (cut: bool)
-  (k: Cbor.raw_data_item)
+  (k: cbor)
   (#ty: typ)
   (#target: Type)
-  (#target_prop: target -> prop)
+  (#target_prop: target -> bool)
   (p: parser_spec ty target target_prop)
-  (target_size: target -> GTot nat {
+  (target_size: target -> Tot nat {
     forall x . target_size x == 1
   })
 : Tot (map_group_parser_spec (map_group_match_item_for cut k ty) (t_literal k) target_size target_prop)
 = fun x ->
-  let Some v = Cbor.list_ghost_assoc k x in
-  Cbor.cbor_map_equiv (Cbor.cbor_map_of_list x) (Cbor.cbor_map_of_list [k, v]);
-  Cbor.cbor_map_length_of_list [k, v];
+  let Some v = cbor_map_get x k in
+  cbor_map_equiv x (cbor_map_singleton k v);
   p v
 
 let map_group_serializer_spec_match_item_for
   (cut: bool)
-  (k: Cbor.raw_data_item)
+  (k: cbor)
   (#ty: typ)
   (#target: Type)
-  (#target_prop: target -> prop)
+  (#target_prop: target -> bool)
   (#p: parser_spec ty target target_prop)
   (s: serializer_spec p)
-  (target_size: target -> GTot nat {
+  (target_size: target -> Tot nat {
     forall x . target_size x == 1
   })
 : Tot (map_group_serializer_spec (map_group_parser_spec_match_item_for cut k p target_size))
 = fun x ->
   map_group_footprint_match_item_for cut k ty;
   let v = s x in
-  let res = [k, v] in
-  let mres = Cbor.cbor_map_of_list res in
-  Cbor.cbor_map_equiv mres (Cbor.cbor_map_singleton k v);
-  let MapGroupDet _ rem = apply_map_group_det (map_group_match_item_for cut k ty) mres in
-  Cbor.cbor_map_equiv rem Cbor.cbor_map_empty;
+  let res = cbor_map_singleton k v in
+  let MapGroupDet _ rem = apply_map_group_det (map_group_match_item_for cut k ty) res in
+  cbor_map_equiv rem cbor_map_empty;
   res
 
 let mg_spec_match_item_for_size
   (target: Type)
   (x: target)
-: GTot nat
+: Tot nat
 = 1
 
 let mg_spec_match_item_for
   (cut: bool)
-  (k: Cbor.raw_data_item)
+  (k: cbor)
   (#ty: typ)
   (#target: Type)
-  (p: spec ty target)
-: Tot (mg_spec (map_group_match_item_for cut k ty) (t_literal k) target)
+  (#inj: bool)
+  (p: spec ty target inj)
+: Tot (mg_spec (map_group_match_item_for cut k ty) (t_literal k) target inj)
 = {
   mg_size = mg_spec_match_item_for_size target;
   mg_serializable = p.serializable;
   mg_parser = map_group_parser_spec_match_item_for cut k p.parser _;
   mg_serializer = map_group_serializer_spec_match_item_for cut k p.serializer _;
+  mg_inj = ();
 }
+
+val map_group_concat_footprint_disjoint
+  (source1: det_map_group)
+  (source_fp1: typ)
+  (source2: det_map_group)
+  (source_fp2: typ {
+    map_group_footprint source1 source_fp1 /\
+    map_group_footprint source2 source_fp2 /\
+    typ_disjoint source_fp1 source_fp2
+  })
+  (m: cbor_map)
+: Lemma
+  (requires (
+    map_group_serializer_spec_arg_prop (map_group_concat source1 source2) (source_fp1 `t_choice` source_fp2) m
+  ))
+  (ensures (
+    let m1 = cbor_map_filter (matches_map_group_entry source_fp1 any) m in
+    let m2 = cbor_map_filter (matches_map_group_entry source_fp2 any) m in
+    cbor_map_disjoint m1 m2 /\
+    cbor_map_union m1 m2 == m /\
+    apply_map_group_det source1 m1 == MapGroupDet m1 cbor_map_empty /\
+    apply_map_group_det source1 m == MapGroupDet m1 m2 /\
+    apply_map_group_det source2 m2 == MapGroupDet m2 cbor_map_empty
+  ))
 
 val map_group_parser_spec_concat
   (#source1: det_map_group)
   (#source_fp1: typ)
   (#target1: Type)
-  (#target_size1: target1 -> GTot nat)
-  (#target_prop1: target1 -> prop)
+  (#target_size1: target1 -> Tot nat)
+  (#target_prop1: target1 -> bool)
   (p1: map_group_parser_spec source1 source_fp1 target_size1 target_prop1)
   (#source2: det_map_group)
   (#source_fp2: typ)
   (#target2: Type)
-  (#target_size2: target2 -> GTot nat)
-  (#target_prop2: target2 -> prop)
+  (#target_size2: target2 -> Tot nat)
+  (#target_prop2: target2 -> bool)
   (p2: map_group_parser_spec source2 source_fp2 target_size2 target_prop2)
-  (target_size: (target1 & target2) -> GTot nat {
+  (target_size: (target1 & target2) -> Tot nat {
     map_group_footprint source1 source_fp1 /\
     map_group_footprint source2 source_fp2 /\
     typ_disjoint source_fp1 source_fp2 /\
     (forall x . target_size x == target_size1 (fst x) + target_size2 (snd x))
   })
-  (target_prop: (target1 & target2) -> prop {
+  (target_prop: (target1 & target2) -> bool {
     forall x . target_prop x <==> (target_prop1 (fst x) /\ target_prop2 (snd x))
   })
 : Tot (map_group_parser_spec (map_group_concat source1 source2) (source_fp1 `t_choice` source_fp2) target_size target_prop)
@@ -1152,35 +1252,33 @@ val map_group_parser_spec_concat_eq
   (#source1: det_map_group)
   (#source_fp1: typ)
   (#target1: Type)
-  (#target_size1: target1 -> GTot nat)
-  (#target_prop1: target1 -> prop)
+  (#target_size1: target1 -> Tot nat)
+  (#target_prop1: target1 -> bool)
   (p1: map_group_parser_spec source1 source_fp1 target_size1 target_prop1)
   (#source2: det_map_group)
   (#source_fp2: typ)
   (#target2: Type)
-  (#target_size2: target2 -> GTot nat)
-  (#target_prop2: target2 -> prop)
+  (#target_size2: target2 -> Tot nat)
+  (#target_prop2: target2 -> bool)
   (p2: map_group_parser_spec source2 source_fp2 target_size2 target_prop2)
-  (target_size: (target1 & target2) -> GTot nat {
+  (target_size: (target1 & target2) -> Tot nat {
     map_group_footprint source1 source_fp1 /\
     map_group_footprint source2 source_fp2 /\
     typ_disjoint source_fp1 source_fp2 /\
     (forall x . target_size x == target_size1 (fst x) + target_size2 (snd x))
   })
-  (target_prop: (target1 & target2) -> prop {
+  (target_prop: (target1 & target2) -> bool {
     forall x . target_prop x <==> (target_prop1 (fst x) /\ target_prop2 (snd x))
   })
   (l: map_group_parser_spec_arg (map_group_concat source1 source2) (source_fp1 `t_choice` source_fp2))
 : Lemma
-  (exists (f1: _ -> bool) (f2: _ -> bool) .
-    (forall x . f1 x == matches_map_group_entry source_fp1 any x) /\
-    (forall x . f2 x == matches_map_group_entry source_fp2 any x) /\ (
-    let l1 = List.Tot.filter f1 l in
-    let l2 = List.Tot.filter f2 l in
+  (
+    let l1 = cbor_map_filter (matches_map_group_entry source_fp1 any) l in
+    let l2 = cbor_map_filter (matches_map_group_entry source_fp2 any) l in
     map_group_parser_spec_arg_prop source1 source_fp1 l1 /\
     map_group_parser_spec_arg_prop source2 source_fp2 l2 /\
     map_group_parser_spec_concat p1 p2 target_size target_prop l == (p1 l1, p2 l2)
-  ))
+  )
   [SMTPat (map_group_parser_spec_concat p1 p2 target_size target_prop l)]
 
 let orp (#t: Type) (p1 p2: t -> bool) (x: t) : bool =
@@ -1191,24 +1289,24 @@ let map_group_serializer_spec_concat
   (#source1: det_map_group)
   (#source_fp1: typ)
   (#target1: Type)
-  (#target_size1: target1 -> GTot nat)
-  (#target_prop1: target1 -> prop)
+  (#target_size1: target1 -> Tot nat)
+  (#target_prop1: target1 -> bool)
   (#p1: map_group_parser_spec source1 source_fp1 target_size1 target_prop1)
   (s1: map_group_serializer_spec p1)
   (#source2: det_map_group)
   (#source_fp2: typ)
   (#target2: Type)
-  (#target_size2: target2 -> GTot nat)
-  (#target_prop2: target2 -> prop)
+  (#target_size2: target2 -> Tot nat)
+  (#target_prop2: target2 -> bool)
   (#p2: map_group_parser_spec source2 source_fp2 target_size2 target_prop2)
   (s2: map_group_serializer_spec p2)
-  (target_size: (target1 & target2) -> GTot nat {
+  (target_size: (target1 & target2) -> Tot nat {
     map_group_footprint source1 source_fp1 /\
     map_group_footprint source2 source_fp2 /\
     typ_disjoint source_fp1 source_fp2 /\
     (forall x . target_size x == target_size1 (fst x) + target_size2 (snd x))
   })
-  (target_prop: (target1 & target2) -> prop {
+  (target_prop: (target1 & target2) -> bool {
     forall x . target_prop x <==> (target_prop1 (fst x) /\ target_prop2 (snd x))
   })
 : Tot (map_group_serializer_spec (map_group_parser_spec_concat p1 p2 target_size target_prop))
@@ -1217,111 +1315,128 @@ let map_group_serializer_spec_concat
     let (x1, x2) = x in
     let l1 = s1 x1 in
     let l2 = s2 x2 in
-    let res = l1 `List.Tot.append` l2 in
-    map_group_footprint_concat_consumes_all source1 source2 source_fp1 source_fp2 (Cbor.cbor_map_of_list l1) (Cbor.cbor_map_of_list l2);
-    List.Tot.append_length l1 l2;
-    assert (Cbor.cbor_map_in_footprint (Cbor.cbor_map_of_list l1) (source_fp1 `t_choice` source_fp2));
-    assert (Cbor.cbor_map_in_footprint (Cbor.cbor_map_of_list l2) (source_fp1 `t_choice` source_fp2));
-    assert (Cbor.cbor_map_in_footprint (Cbor.cbor_map_of_list l1 `Cbor.cbor_map_union` Cbor.cbor_map_of_list l2) (source_fp1 `t_choice` source_fp2));
-    Cbor.cbor_map_of_list_append l1 l2;
-    Cbor.cbor_map_length_of_list (l1 `List.Tot.append` l2);
+    let res = l1 `cbor_map_union` l2 in
+    assert (cbor_map_disjoint l1 l2);
+    map_group_footprint_concat_consumes_all source1 source2 source_fp1 source_fp2 (l1) (l2);
+    assert (cbor_map_in_footprint (l1) (source_fp1 `t_choice` source_fp2));
+    assert (cbor_map_in_footprint (l2) (source_fp1 `t_choice` source_fp2));
+    assert (cbor_map_in_footprint (l1 `cbor_map_union` l2) (source_fp1 `t_choice` source_fp2));
     assert (map_group_serializer_spec_arg_prop (source1 `map_group_concat` source2) (source_fp1 `t_choice` source_fp2) res);
-    let prf
-      (f1 : _ -> bool) (f2 : _ -> bool)
-    : Lemma
-      (requires (
-        (forall x . f1 x == matches_map_group_entry source_fp1 any x) /\
-        (forall x . f2 x == matches_map_group_entry source_fp2 any x)
-      ))
-      (ensures (
-        (forall x . (f1 `orp` f2) x == matches_map_group_entry (source_fp1 `t_choice` source_fp2) any x) /\
-        l1 == List.Tot.filter f1 res /\
-        l2 == List.Tot.filter f2 res
-      ))
-    = assert (forall x . (f1 `orp` f2) x == matches_map_group_entry (source_fp1 `t_choice` source_fp2) any x);
-      list_filter_append f1 l1 l2;
-      list_forall_memP_filter f1 l1;
-      list_filter_for_none f1 l2;
-      List.Tot.append_l_nil l1;
-      list_filter_for_none f2 l1;
-      list_forall_memP_filter f2 l2;
-      list_filter_append f2 l1 l2
-    in
-    Classical.forall_intro_2 (fun f1 -> Classical.move_requires (prf f1));
+    let f1 = matches_map_group_entry source_fp1 any in
+    let f2 = matches_map_group_entry source_fp2 any in
+    let f = matches_map_group_entry (source_fp1 `t_choice` source_fp2) any in
+    cbor_map_filter_ext (f1 `orp` f2) f res;
+    assert (cbor_map_equal l1 (cbor_map_filter f1 l1));
+    assert (cbor_map_equal cbor_map_empty (cbor_map_filter f1 l2));
+    assert (cbor_map_equal l1 (cbor_map_filter f1 res));
+    assert (cbor_map_equal l2 (cbor_map_filter f2 l2));
+    assert (cbor_map_equal cbor_map_empty (cbor_map_filter f2 l1));
+    assert (cbor_map_equal l2 (cbor_map_filter f2 res));
     assert (map_group_parser_spec_concat p1 p2 target_size target_prop res == x);
+    cbor_map_length_disjoint_union l1 l2;
     res
 
 let mg_spec_concat_size
   (#source1: det_map_group)
   (#source_fp1: typ)
   (#target1: Type)
-  (p1: mg_spec source1 source_fp1 target1)
+  (#inj1: bool)
+  (p1: mg_spec source1 source_fp1 target1 inj1)
   (#source2: det_map_group)
   (#source_fp2: typ)
   (#target2: Type)
-  (p2: mg_spec source2 source_fp2 target2)
+  (#inj2: bool)
+  (p2: mg_spec source2 source_fp2 target2 inj2)
   (x: (target1 & target2))
-: GTot nat
+: Tot nat
 = p1.mg_size (fst x) + p2.mg_size (snd x)
 
 let mg_spec_concat_serializable
   (#source1: det_map_group)
   (#source_fp1: typ)
   (#target1: Type)
-  (p1: mg_spec source1 source_fp1 target1)
+  (#inj1: bool)
+  (p1: mg_spec source1 source_fp1 target1 inj1)
   (#source2: det_map_group)
   (#source_fp2: typ)
   (#target2: Type)
-  (p2: mg_spec source2 source_fp2 target2)
+  (#inj2: bool)
+  (p2: mg_spec source2 source_fp2 target2 inj2)
   (x: (target1 & target2))
-: Tot prop
-= p1.mg_serializable (fst x) /\ p2.mg_serializable (snd x)
+: Tot bool
+= p1.mg_serializable (fst x) && p2.mg_serializable (snd x)
+
+let mg_spec_concat_inj
+  (#source1: det_map_group)
+  (#source_fp1: typ)
+  (#target1: Type)
+  (#inj1: bool)
+  (p1: mg_spec source1 source_fp1 target1 inj1)
+  (#source2: det_map_group)
+  (#source_fp2: typ)
+  (#target2: Type)
+  (#inj2: bool)
+  (p2: mg_spec source2 source_fp2 target2 inj2 {
+    map_group_footprint source1 source_fp1 /\
+    map_group_footprint source2 source_fp2 /\
+    typ_disjoint source_fp1 source_fp2
+  })
+  (m: cbor_map { map_group_serializer_spec_arg_prop (map_group_concat source1 source2) (source_fp1 `t_choice` source_fp2) m })
+: Lemma
+  (requires (inj1 && inj2))
+  (ensures (
+    map_group_serializer_spec_concat p1.mg_serializer p2.mg_serializer (mg_spec_concat_size p1 p2) (mg_spec_concat_serializable p1 p2) (map_group_parser_spec_concat p1.mg_parser p2.mg_parser (mg_spec_concat_size p1 p2) (mg_spec_concat_serializable p1 p2) m) == m
+  ))
+= map_group_concat_footprint_disjoint source1 source_fp1 source2 source_fp2 m
 
 let mg_spec_concat
   (#source1: det_map_group)
   (#source_fp1: typ)
   (#target1: Type)
-  (p1: mg_spec source1 source_fp1 target1)
+  (#inj1: bool)
+  (p1: mg_spec source1 source_fp1 target1 inj1)
   (#source2: det_map_group)
   (#source_fp2: typ)
   (#target2: Type)
-  (p2: mg_spec source2 source_fp2 target2 {
+  (#inj2: bool)
+  (p2: mg_spec source2 source_fp2 target2 inj2 {
     map_group_footprint source1 source_fp1 /\
     map_group_footprint source2 source_fp2 /\
     typ_disjoint source_fp1 source_fp2
   })
-: Tot (mg_spec (map_group_concat source1 source2) (source_fp1 `t_choice` source_fp2) (target1 & target2))
+: Tot (mg_spec (map_group_concat source1 source2) (source_fp1 `t_choice` source_fp2) (target1 & target2) (inj1 && inj2))
 = {
   mg_size = mg_spec_concat_size p1 p2;
   mg_serializable = mg_spec_concat_serializable p1 p2;
   mg_parser = map_group_parser_spec_concat p1.mg_parser p2.mg_parser _ _;
   mg_serializer = map_group_serializer_spec_concat p1.mg_serializer p2.mg_serializer _ _;
+  mg_inj = Classical.forall_intro (Classical.move_requires (mg_spec_concat_inj p1 p2));
 }
 
 val map_group_parser_spec_choice
   (#source1: det_map_group)
   (#source_fp1: typ)
   (#target1: Type)
-  (#target_size1: target1 -> GTot nat)
-  (#target_prop1: target1 -> prop)
+  (#target_size1: target1 -> Tot nat)
+  (#target_prop1: target1 -> bool)
   (p1: map_group_parser_spec source1 source_fp1 target_size1 target_prop1 {
     map_group_footprint source1 source_fp1
   })
   (#source2: det_map_group)
   (#source_fp2: typ)
   (#target2: Type)
-  (#target_size2: target2 -> GTot nat)
-  (#target_prop2: target2 -> prop)
+  (#target_size2: target2 -> Tot nat)
+  (#target_prop2: target2 -> bool)
   (p2: map_group_parser_spec source2 source_fp2 target_size2 target_prop2 {
     map_group_footprint source2 source_fp2
   })
-  (target_size: (target1 `either` target2) -> GTot nat {
+  (target_size: (target1 `either` target2) -> Tot nat {
     forall x . target_size x == begin match x with
     | Inl y -> target_size1 y
     | Inr y -> target_size2 y
     end
   })
-  (target_prop: (target1 `either` target2) -> prop {
+  (target_prop: (target1 `either` target2) -> bool {
     forall x . target_prop x <==> begin match x with
     | Inl x1 -> target_prop1 x1
     | Inr x2 -> target_prop2 x2
@@ -1333,26 +1448,26 @@ val map_group_parser_spec_choice_eq
   (#source1: det_map_group)
   (#source_fp1: typ)
   (#target1: Type)
-  (#target_size1: target1 -> GTot nat)
-  (#target_prop1: target1 -> prop)
+  (#target_size1: target1 -> Tot nat)
+  (#target_prop1: target1 -> bool)
   (p1: map_group_parser_spec source1 source_fp1 target_size1 target_prop1 {
     map_group_footprint source1 source_fp1
   })
   (#source2: det_map_group)
   (#source_fp2: typ)
   (#target2: Type)
-  (#target_size2: target2 -> GTot nat)
-  (#target_prop2: target2 -> prop)
+  (#target_size2: target2 -> Tot nat)
+  (#target_prop2: target2 -> bool)
   (p2: map_group_parser_spec source2 source_fp2 target_size2 target_prop2 {
     map_group_footprint source2 source_fp2
   })
-  (target_size: (target1 `either` target2) -> GTot nat {
+  (target_size: (target1 `either` target2) -> Tot nat {
     forall x . target_size x == begin match x with
     | Inl y -> target_size1 y
     | Inr y -> target_size2 y
     end
   })
-  (target_prop: (target1 `either` target2) -> prop {
+  (target_prop: (target1 `either` target2) -> bool {
     forall x . target_prop x <==> begin match x with
     | Inl x1 -> target_prop1 x1
     | Inr x2 -> target_prop2 x2
@@ -1363,23 +1478,22 @@ val map_group_parser_spec_choice_eq
     (requires True)
     (ensures (
         let l' = map_group_parser_spec_choice p1 p2 target_size target_prop l in
-        exists (f1: _ -> bool) (f2: _ -> bool) .
-        (forall x . f1 x == matches_map_group_entry source_fp1 any x) /\
-        (forall x . f2 x == matches_map_group_entry source_fp2 any x) /\ (
-        let l1 = List.Tot.filter f1 l in
-        let l2 = List.Tot.filter f2 l in
-        let test = MapGroupDet? (apply_map_group_det source1 (Cbor.cbor_map_of_list l1)) in
-        Cbor.cbor_map_of_list l1 == Cbor.cbor_map_filter (matches_map_group_entry source_fp1 any) (Cbor.cbor_map_of_list l) /\
-        Cbor.cbor_map_of_list l2 == Cbor.cbor_map_filter (matches_map_group_entry source_fp2 any) (Cbor.cbor_map_of_list l) /\
+        let f1 = matches_map_group_entry source_fp1 any in
+        let f2 = matches_map_group_entry source_fp2 any in
+        let l1 = cbor_map_filter f1 l in
+        let l2 = cbor_map_filter f2 l in
+        let test = MapGroupDet? (apply_map_group_det source1 (l1)) in
+        l1 == cbor_map_filter (matches_map_group_entry source_fp1 any) (l) /\
+        l2 == cbor_map_filter (matches_map_group_entry source_fp2 any) (l) /\
         (test ==> (
           map_group_parser_spec_arg_prop source1 source_fp1 l1 /\
           (l' <: (target1 `either` target2)) == Inl (p1 l1)
         )) /\
-        (~ test ==> (
+        ((~ test) ==> (
           map_group_parser_spec_arg_prop source2 source_fp2 l2 /\
           (l' <: (target1 `either` target2)) == Inr (p2 l2)
         ))
-    )))
+    ))
     [SMTPat (map_group_parser_spec_choice p1 p2 target_size target_prop l)]
 
 #restart-solver
@@ -1387,8 +1501,8 @@ let map_group_serializer_spec_choice
   (#source1: det_map_group)
   (#source_fp1: typ)
   (#target1: Type)
-  (#target_size1: target1 -> GTot nat)
-  (#target_prop1: target1 -> prop)
+  (#target_size1: target1 -> Tot nat)
+  (#target_prop1: target1 -> bool)
   (#p1: map_group_parser_spec source1 source_fp1 target_size1 target_prop1)
   (s1: map_group_serializer_spec p1 {
     map_group_footprint source1 source_fp1
@@ -1396,20 +1510,20 @@ let map_group_serializer_spec_choice
   (#source2: det_map_group)
   (#source_fp2: typ)
   (#target2: Type)
-  (#target_size2: target2 -> GTot nat)
-  (#target_prop2: target2 -> prop)
+  (#target_size2: target2 -> Tot nat)
+  (#target_prop2: target2 -> bool)
   (#p2: map_group_parser_spec source2 source_fp2 target_size2 target_prop2)
   (s2: map_group_serializer_spec p2 {
     map_group_footprint source2 source_fp2 /\
     map_group_choice_compatible source1 source2
   })
-  (target_size: (target1 `either` target2) -> GTot nat {
+  (target_size: (target1 `either` target2) -> Tot nat {
     forall x . target_size x == begin match x with
     | Inl y -> target_size1 y
     | Inr y -> target_size2 y
     end
   })
-  (target_prop: (target1 `either` target2) -> prop {
+  (target_prop: (target1 `either` target2) -> bool {
     forall x . target_prop x <==> begin match x with
     | Inl x1 -> target_prop1 x1
     | Inr x2 -> target_prop2 x2
@@ -1417,36 +1531,45 @@ let map_group_serializer_spec_choice
   })  
 : Tot (map_group_serializer_spec (map_group_parser_spec_choice p1 p2 target_size target_prop))
 = fun x ->
-    let res : list (Cbor.raw_data_item & Cbor.raw_data_item) =
+    let res : cbor_map =
       match x with
       | Inl y -> s1 y
       | Inr y -> s2 y
     in
     assert (map_group_serializer_spec_arg_prop (source1 `map_group_choice` source2) (source_fp1 `t_choice` source_fp2) res);
-    assert (target_size x == List.Tot.length res);
-    Classical.forall_intro (fun f -> Classical.move_requires (list_forall_memP_filter f) res);
-    let _ : squash (map_group_parser_spec_choice p1 p2 target_size target_prop res == x) =
+    assert (target_size x == cbor_map_length res);
+    let res1 = cbor_map_filter (matches_map_group_entry source_fp1 any) res in
+    let f () : Lemma (map_group_parser_spec_choice p1 p2 target_size target_prop res == x) =
       match x with
-      | Inl y -> ()
+      | Inl y ->
+        assert (res1 `cbor_map_equal` res);
+        map_group_parser_spec_choice_eq p1 p2 target_size target_prop res;
+        assert (map_group_parser_spec_choice p1 p2 target_size target_prop res == x)
       | Inr y ->
-        assert (MapGroupDet? (apply_map_group_det source2 (Cbor.cbor_map_of_list res)));
-        assert (MapGroupFail? (apply_map_group_det source1 (Cbor.cbor_map_of_list res)));
-        map_group_footprint_is_consumed_Cbor.cbor_map_of_list source1 source_fp1 res;
+        assert (cbor_map_filter (matches_map_group_entry source_fp2 any) res `cbor_map_equal` res);
+        map_group_parser_spec_choice_eq p1 p2 target_size target_prop res;
+        assert (MapGroupDet? (apply_map_group_det source2 (res)));
+        assert (MapGroupFail? (apply_map_group_det source1 (res)));
+        map_group_footprint_elim source1 source_fp1 res1 (cbor_map_sub res res1);
+        assert (MapGroupFail? (apply_map_group_det source1 (res1)));
         assert (map_group_parser_spec_choice p1 p2 target_size target_prop res == x)
     in
+    f ();
     res
 
 let mg_spec_choice_size
   (#source1: det_map_group)
   (#source_fp1: typ)
   (#target1: Type)
-  (p1: mg_spec source1 source_fp1 target1)
+  (#inj1: bool)
+  (p1: mg_spec source1 source_fp1 target1 inj1)
   (#source2: det_map_group)
   (#source_fp2: typ)
   (#target2: Type)
-  (p2: mg_spec source2 source_fp2 target2)
+  (#inj2: bool)
+  (p2: mg_spec source2 source_fp2 target2 inj2)
   (x: either target1 target2)
-: GTot nat
+: Tot nat
 = match x with
   | Inl x1 -> p1.mg_size x1
   | Inr x2 -> p2.mg_size x2
@@ -1455,205 +1578,536 @@ let mg_spec_choice_serializable
   (#source1: det_map_group)
   (#source_fp1: typ)
   (#target1: Type)
-  (p1: mg_spec source1 source_fp1 target1)
+  (#inj1: bool)
+  (p1: mg_spec source1 source_fp1 target1 inj1)
   (#source2: det_map_group)
   (#source_fp2: typ)
   (#target2: Type)
-  (p2: mg_spec source2 source_fp2 target2)
+  (#inj2: bool)
+  (p2: mg_spec source2 source_fp2 target2 inj2)
   (x: either target1 target2)
-: Tot prop
+: Tot bool
 = match x with
   | Inl x1 -> p1.mg_serializable x1
   | Inr x2 -> p2.mg_serializable x2
 
-let mg_spec_choice
+let mg_spec_choice_inj
   (#source1: det_map_group)
   (#source_fp1: typ)
   (#target1: Type)
-  (p1: mg_spec source1 source_fp1 target1 {
+  (#inj1: bool)
+  (p1: mg_spec source1 source_fp1 target1 inj1 {
     map_group_footprint source1 source_fp1
   })
   (#source2: det_map_group)
   (#source_fp2: typ)
   (#target2: Type)
-  (p2: mg_spec source2 source_fp2 target2 {
+  (#inj2: bool)
+  (p2: mg_spec source2 source_fp2 target2 inj2 {
     map_group_footprint source2 source_fp2 /\
     map_group_choice_compatible source1 source2
   })
-: Tot (mg_spec (map_group_choice source1 source2) (source_fp1 `t_choice` source_fp2) (either target1 target2))
+  (c: cbor_map { map_group_serializer_spec_arg_prop (map_group_choice source1 source2) (t_choice source_fp1 source_fp2) c })
+: Lemma
+  (requires (inj1 && inj2))
+  (ensures map_group_serializer_spec_choice p1.mg_serializer p2.mg_serializer (mg_spec_choice_size p1 p2) (mg_spec_choice_serializable p1 p2) (map_group_parser_spec_choice p1.mg_parser p2.mg_parser (mg_spec_choice_size p1 p2) (mg_spec_choice_serializable p1 p2) c) == c)
+= let f1 = matches_map_group_entry source_fp1 any in
+  cbor_map_split f1 c;
+  let c1 = cbor_map_filter f1 c in
+  let c1' = cbor_map_filter (U.notp f1) c in
+  map_group_footprint_elim source1 source_fp1 c1 c1';
+  match apply_map_group_det source1 c1 with
+  | MapGroupDet _ _ ->
+    assert (cbor_map_equal c1' cbor_map_empty);
+    assert (c1 == c)
+  | MapGroupFail ->
+    let f2 = matches_map_group_entry source_fp2 any in
+    cbor_map_split f2 c;
+    let c2 = cbor_map_filter f2 c in
+    let c2' = cbor_map_filter (U.notp f2) c in
+    map_group_footprint_elim source2 source_fp2 c2 c2';
+    assert (cbor_map_equal c2' cbor_map_empty);
+    assert (c2 == c)
+
+let mg_spec_choice
+  (#source1: det_map_group)
+  (#source_fp1: typ)
+  (#target1: Type)
+  (#inj1: bool)
+  (p1: mg_spec source1 source_fp1 target1 inj1 {
+    map_group_footprint source1 source_fp1
+  })
+  (#source2: det_map_group)
+  (#source_fp2: typ)
+  (#target2: Type)
+  (#inj2: bool)
+  (p2: mg_spec source2 source_fp2 target2 inj2 {
+    map_group_footprint source2 source_fp2 /\
+    map_group_choice_compatible source1 source2
+  })
+: Tot (mg_spec (map_group_choice source1 source2) (source_fp1 `t_choice` source_fp2) (either target1 target2) (inj1 && inj2))
 = {
   mg_size = mg_spec_choice_size p1 p2;
   mg_serializable = mg_spec_choice_serializable p1 p2;
   mg_parser = map_group_parser_spec_choice p1.mg_parser p2.mg_parser _ _;
   mg_serializer = map_group_serializer_spec_choice p1.mg_serializer p2.mg_serializer _ _;
+  mg_inj = Classical.forall_intro (Classical.move_requires (mg_spec_choice_inj p1 p2));
 }
 
-(*
-let rec map_group_parser_spec_zero_or_more'
-  (#source: det_map_group)
-  (#target: Type)
-  (#target_size: target -> nat)
-  (p: map_group_parser_spec source target_size {
-    map_group3_concat_unique_strong source source
-  })
-  (target_size' : list target -> nat {
-    forall (l: list target) . target_size' l == (if Nil? l then 0 else target_size (List.Tot.hd l) + target_size' (List.Tot.tl l))
-  })
-  (x: map_group_parser_spec_arg (map_group3_zero_or_more source) target_size')
-: GTot (map_group_parser_spec_ret (map_group3_zero_or_more source) target_size' x)
-  (decreases (List.Tot.length x))
-= match source x with
-  | None ->
-    assert (x == []);
-    let res : list target = [] in
-    assert (Nil? res);
-    assert (target_size' res == 0);
-    res
-  | Some (l1, l2) ->
-    if Nil? l1
-    then []
+let map_group_footprint_disjoint_productive_choice_compatible
+  (source1 source2: det_map_group)
+  (source_fp1 source_fp2: typ)
+: Lemma
+  (requires (
+    map_group_footprint source1 source_fp1 /\
+    map_group_footprint source2 source_fp2 /\
+    typ_disjoint source_fp1 source_fp2 /\
+    MapGroupFail? (apply_map_group_det source1 cbor_map_empty)
+  ))
+  (ensures (
+    map_group_choice_compatible source1 source2
+  ))
+= map_group_choice_compatible_intro source1 source2 (fun x ->
+    if x = cbor_map_empty
+    then ()
     else begin
-      map_group3_concat_unique_weak_zero_or_more_right source source;
-      List.Tot.append_length l1 l2;
-      let q = map_group_parser_spec_zero_or_more' p target_size' l2 in
-      p l1 :: q
+      map_group_footprint_consumes_all source2 source_fp2 x;
+      map_group_footprint_consumed_disjoint source2 source_fp2 source_fp1 x;
+      map_group_footprint_elim source1 source_fp1 cbor_map_empty x
     end
+  )
 
-let map_group_parser_spec_zero_or_more
-  (#source: det_map_group)
-  (#target: Type)
-  (#target_size: target -> nat)
-  (p: map_group_parser_spec source target_size {
-    map_group3_concat_unique_strong source source
-  })
-  (target_size' : list target -> nat {
-    forall (l: list target) . target_size' l == (if Nil? l then 0 else target_size (List.Tot.hd l) + target_size' (List.Tot.tl l))
-  })
-: Tot (map_group_parser_spec (map_group3_zero_or_more source) target_size')
-= map_group_parser_spec_zero_or_more' p target_size'
-
-let nonempty_map_group : Type0 =
-  (a: map_group {
-    forall l . match a l with
-    | Some (consumed, _) -> Cons? consumed
-    | _ -> True
-  })
-
-let rec map_group_serializer_spec_zero_or_more'
-  (#source: nonempty_map_group)
-  (#target: Type)
-  (#target_size: target -> nat)
-  (#p: map_group_parser_spec source target_size)
-  (s: map_group_serializer_spec p {
-    map_group3_concat_unique_strong source source
-  })
-  (target_size' : list target -> nat {
-    forall (l: list target) . target_size' l == (if Nil? l then 0 else target_size (List.Tot.hd l) + target_size' (List.Tot.tl l))
-  })
-  (x: list target)
-: GTot (y: map_group_parser_spec_arg (map_group3_zero_or_more source) target_size' {
-    map_group_parser_spec_zero_or_more p target_size' y == x
-  })
-  (decreases x)
+let map_group_size_zero_or_one
+  (#target1: Type)
+  (sz: target1 -> nat)
+  (x: option target1)
+: nat
 = match x with
-  | [] -> []
+  | None -> 0
+  | Some x -> sz x
+
+let map_group_serializable_zero_or_one
+  (#target1: Type)
+  (sz: target1 -> bool)
+  (x: option target1)
+: bool
+= match x with
+  | None -> true
+  | Some x -> sz x
+
+let mg_spec_zero_or_one
+  (#source1: det_map_group)
+  (#source_fp1: typ)
+  (#target1: Type)
+  (#inj1: bool)
+  (p1: mg_spec source1 source_fp1 target1 inj1 {
+    map_group_footprint source1 source_fp1 /\
+    MapGroupFail? (apply_map_group_det source1 cbor_map_empty)
+  })
+: Tot (mg_spec (map_group_zero_or_one source1) source_fp1 (option target1) inj1)
+= map_group_footprint_disjoint_productive_choice_compatible source1 map_group_nop source_fp1 t_always_false;
+  mg_spec_ext
+    (mg_spec_bij
+      (mg_spec_choice p1 mg_spec_nop)
+      {
+        bij_from_to = (fun x -> match x with Inl x -> Some x | _ -> None);
+        bij_to_from = (fun x -> match x with Some x -> Inl x | _ -> Inr ());
+        bij_from_to_from = ();
+        bij_to_from_to = ();
+      }
+    )
+    source_fp1
+    (map_group_size_zero_or_one p1.mg_size)
+    (map_group_serializable_zero_or_one p1.mg_serializable)
+
+let map_group_zero_or_more_match_item_length
+  (#tkey #tvalue: Type)
+  (#key: typ)
+  (pkey: spec key tkey true)
+  (x: Map.t pkey tvalue)
+: Tot nat
+= Map.length x
+
+let value_serializable
+  (#tkey #tvalue: Type)
+  (#inj: bool)
+  (#value: typ)
+  (pvalue: spec value tvalue inj)
+  (x: (tkey & tvalue))
+: Tot bool
+= pvalue.serializable (snd x)
+
+let map_group_zero_or_more_match_item_parser_op
+  (#tkey #tvalue: Type)
+  (#key #value: typ)
+  (pkey: spec key tkey true)
+  (#inj: bool)
+  (pvalue: spec value tvalue inj)
+  (m: map_group_parser_spec_arg (map_group_zero_or_more (map_group_match_item false key value)) key)
+  (accu: Map.t pkey tvalue)
+  (x: cbor)
+: Tot (Map.t pkey tvalue)
+= match cbor_map_get m x with
+  | None -> accu
+  | Some y ->
+    if value y
+    then Map.union accu (Map.singleton _ (pkey.parser x) (pvalue.parser y))
+    else accu
+
+let map_group_zero_or_more_match_item_parser_op_comm
+  (#tkey #tvalue: Type)
+  (#key #value: typ)
+  (pkey: spec key tkey true)
+  (#inj: bool)
+  (pvalue: spec value tvalue inj)
+  (m: map_group_parser_spec_arg (map_group_zero_or_more (map_group_match_item false key value)) key)
+  (accu: Map.t pkey tvalue)
+  (x1 x2: cbor)
+: Lemma
+  (ensures (map_group_zero_or_more_match_item_parser_op pkey pvalue m (map_group_zero_or_more_match_item_parser_op pkey pvalue m accu x1) x2 `Map.equal` map_group_zero_or_more_match_item_parser_op pkey pvalue m (map_group_zero_or_more_match_item_parser_op pkey pvalue m accu x2) x1
+  ))
+  [SMTPat (map_group_zero_or_more_match_item_parser_op pkey pvalue m (map_group_zero_or_more_match_item_parser_op pkey pvalue m accu x1) x2)]
+= ()
+
+let rec list_fold_map_group_zero_or_more_match_item_parser_op_mem
+  (#tkey #tvalue: Type)
+  (#key #value: typ)
+  (pkey: spec key tkey true)
+  (#inj: bool)
+  (pvalue: spec value tvalue inj)
+  (m: map_group_parser_spec_arg (map_group_zero_or_more (map_group_match_item false key value)) key)
+  (accu: Map.t pkey tvalue)
+  (l: list cbor)
+  (k: tkey)
+  (v: tvalue)
+: Lemma
+  (ensures (
+    let m' = List.Tot.fold_left (map_group_zero_or_more_match_item_parser_op pkey pvalue m) accu l in
+    (Map.get m' k == Some v <==> (match Map.get accu k with
+    | Some v_ -> v_ == v
+    | None ->
+      pkey.serializable k /\
+      List.Tot.memP (pkey.serializer k) l /\
+      begin match cbor_map_get m (pkey.serializer k) with
+      | None -> False
+      | Some v' ->
+        value v' /\
+        pvalue.parser v' == v
+      end
+    ))
+  ))
+  (decreases l)
+=   begin match l with
+    | [] -> ()
+    | a :: q ->
+      list_fold_map_group_zero_or_more_match_item_parser_op_mem pkey pvalue m (map_group_zero_or_more_match_item_parser_op pkey pvalue m accu a) q k v
+    end
+
+let map_group_zero_or_more_match_item_parser_op_length
+  (#tkey #tvalue: Type)
+  (#key #value: typ)
+  (pkey: spec key tkey true)
+  (#inj: bool)
+  (pvalue: spec value tvalue inj)
+  (m: map_group_parser_spec_arg (map_group_zero_or_more (map_group_match_item false key value)) key)
+  (accu: Map.t pkey tvalue)
+  (l: cbor)
+: Lemma
+  (ensures (
+    let m' = (map_group_zero_or_more_match_item_parser_op pkey pvalue m) accu l in
+    Map.length m' <= Map.length accu + 1
+  ))
+= match cbor_map_get m l with
+  | None -> ()
+  | Some y ->
+    if value y
+    then
+      if Map.defined (pkey.parser l) accu
+      then assert (map_group_zero_or_more_match_item_parser_op pkey pvalue m accu l `Map.equal` accu)
+      else Map.length_disjoint_union accu (Map.singleton _ (pkey.parser l) (pvalue.parser y))
+    else ()
+
+let rec list_fold_map_group_zero_or_more_match_item_parser_length
+  (#tkey #tvalue: Type)
+  (#key #value: typ)
+  (pkey: spec key tkey true)
+  (#inj: bool)
+  (pvalue: spec value tvalue inj)
+  (m: map_group_parser_spec_arg (map_group_zero_or_more (map_group_match_item false key value)) key)
+  (accu: Map.t pkey tvalue)
+  (l: list cbor)
+: Lemma
+  (ensures (
+    let m' = List.Tot.fold_left (map_group_zero_or_more_match_item_parser_op pkey pvalue m) accu l in
+    Map.length m' <= Map.length accu + List.Tot.length l
+  ))
+  (decreases l)
+= match l with
+  | [] -> ()
   | a :: q ->
-    map_group3_concat_unique_weak_zero_or_more_right source source;
-    let l1 = s a in
-    let l2 = map_group_serializer_spec_zero_or_more' s target_size' q in
-    let res = l1 `List.Tot.append` l2 in
-    res
+    map_group_zero_or_more_match_item_parser_op_length pkey pvalue m accu a;
+    list_fold_map_group_zero_or_more_match_item_parser_length pkey pvalue m (map_group_zero_or_more_match_item_parser_op pkey pvalue m accu a) q
 
-let map_group_serializer_spec_zero_or_more
-  (#source: nonempty_map_group)
-  (#target: Type)
-  (#target_size: target -> nat)
-  (#p: map_group_parser_spec source target_size)
-  (s: map_group_serializer_spec p {
-    map_group3_concat_unique_strong source source
-  })
-  (target_size' : list target -> nat {
-    forall (l: list target) . target_size' l == (if Nil? l then 0 else target_size (List.Tot.hd l) + target_size' (List.Tot.tl l))
-  })
-: Tot (map_group_serializer_spec (map_group_parser_spec_zero_or_more p target_size'))
-= map_group_serializer_spec_zero_or_more' s target_size'
+let map_group_zero_or_more_match_item_parser'
+  (#tkey #tvalue: Type)
+  (#key #value: typ)
+  (pkey: spec key tkey true)
+  (#inj: bool)
+  (pvalue: spec value tvalue inj)
+  (x: map_group_parser_spec_arg (map_group_zero_or_more (map_group_match_item false key value)) key)
+: Tot (Map.t pkey tvalue)
+= cbor_map_fold (map_group_zero_or_more_match_item_parser_op pkey pvalue x) (Map.empty _ _) x
 
-let nelist (a: Type) : Type0 = (l: list a { Cons? l })
+let map_group_zero_or_more_match_item_parser'_mem
+  (#tkey #tvalue: Type)
+  (#key #value: typ)
+  (pkey: spec key tkey true)
+  (#inj: bool)
+  (pvalue: spec value tvalue inj)
+  (m: map_group_parser_spec_arg (map_group_zero_or_more (map_group_match_item false key value)) key)
+  (kv: (tkey & tvalue))
+: Lemma
+  (ensures (
+    let m' = map_group_zero_or_more_match_item_parser' pkey pvalue m in
+    (Map.mem kv m' <==> (
+      let (k, v) = kv in
+      pkey.serializable k /\
+      exists kv' . cbor_map_mem kv' m /\
+      fst kv' == pkey.serializer k /\
+      value (snd kv') /\
+      pvalue.parser (snd kv') == v
+    ))
+  ))
+  [SMTPat (Map.mem kv (map_group_zero_or_more_match_item_parser' pkey pvalue m))]
+= let l = cbor_map_key_list m in
+  cbor_map_fold_eq (map_group_zero_or_more_match_item_parser_op pkey pvalue m) (Map.empty _ _) m l;
+  list_fold_map_group_zero_or_more_match_item_parser_op_mem pkey pvalue m (Map.empty _ _) l (fst kv) (snd kv)
 
-let map_group_parser_spec_one_or_more
-  (#source: det_map_group)
-  (#target: Type)
-  (#target_size: target -> nat)
-  (p: map_group_parser_spec source target_size {
-    map_group3_concat_unique_strong source source
-  })
-  (target_size1 : list target -> nat {
-    forall (l: list target) . target_size1 l == (if Nil? l then 0 else target_size (List.Tot.hd l) + target_size1 (List.Tot.tl l))
-  })
-  (target_size2 : nelist target -> nat {
-    forall (l: nelist target) . target_size2 l == target_size1 l
-  })
-: Tot (map_group_parser_spec (map_group3_one_or_more source) target_size2)
+let map_group_zero_or_more_match_item_parser'_length
+  (#tkey #tvalue: Type)
+  (#key #value: typ)
+  (pkey: spec key tkey true)
+  (#inj: bool)
+  (pvalue: spec value tvalue inj)
+  (m: map_group_parser_spec_arg (map_group_zero_or_more (map_group_match_item false key value)) key)
+: Lemma
+  (ensures (
+    Map.length (map_group_zero_or_more_match_item_parser' pkey pvalue m) <= cbor_map_length m
+  ))
+  [SMTPat (Map.length (map_group_zero_or_more_match_item_parser' pkey pvalue m))]
+= let l = cbor_map_key_list m in
+  cbor_map_fold_eq (map_group_zero_or_more_match_item_parser_op pkey pvalue m) (Map.empty _ _) m l;
+  list_fold_map_group_zero_or_more_match_item_parser_length pkey pvalue m (Map.empty _ _) l
+
+let map_group_zero_or_more_match_item_parser
+  (#tkey #tvalue: Type)
+  (#key #value: typ)
+  (pkey: spec key tkey true)
+  (#inj: bool)
+  (pvalue: spec value tvalue inj)
+: Tot (map_group_parser_spec (map_group_zero_or_more (map_group_match_item false key value)) key (map_group_zero_or_more_match_item_length pkey) (Map.for_all (value_serializable pvalue)))
+= fun x -> map_group_zero_or_more_match_item_parser' pkey pvalue x
+
+let map_group_zero_or_more_match_item_serializer_op
+  (#tkey #tvalue: Type)
+  (#key #value: typ)
+  (pkey: spec key tkey true)
+  (#inj: bool)
+  (pvalue: spec value tvalue inj)
+  (m: Map.t pkey tvalue { Map.for_all (value_serializable pvalue) m })
+  (accu: cbor_map)
+  (x: tkey)
+: Tot (cbor_map)
+= match Map.get m x with
+  | None -> accu
+  | Some y ->
+    cbor_map_union accu (cbor_map_singleton (pkey.serializer x) (pvalue.serializer y))
+
+let map_group_zero_or_more_match_item_serializer_op_comm
+  (#tkey #tvalue: Type)
+  (#key #value: typ)
+  (pkey: spec key tkey true)
+  (#inj: bool)
+  (pvalue: spec value tvalue inj)
+  (m: Map.t pkey tvalue { Map.for_all (value_serializable pvalue) m })
+  (accu: cbor_map)
+  (x1 x2: tkey)
+: Lemma
+  (ensures (map_group_zero_or_more_match_item_serializer_op pkey pvalue m (map_group_zero_or_more_match_item_serializer_op pkey pvalue m accu x1) x2 `cbor_map_equal` map_group_zero_or_more_match_item_serializer_op pkey pvalue m (map_group_zero_or_more_match_item_serializer_op pkey pvalue m accu x2) x1
+  ))
+  [SMTPat (map_group_zero_or_more_match_item_serializer_op pkey pvalue m (map_group_zero_or_more_match_item_serializer_op pkey pvalue m accu x1) x2)]
+= ()
+
+let rec list_fold_map_group_zero_or_more_match_item_serializer_op_mem
+  (#tkey #tvalue: Type)
+  (#key #value: typ)
+  (pkey: spec key tkey true)
+  (#inj: bool)
+  (pvalue: spec value tvalue inj)
+  (m: Map.t pkey tvalue { Map.for_all (value_serializable pvalue) m })
+  (accu: cbor_map)
+  (l: list tkey)
+  (kv: (cbor & cbor))
+: Lemma
+  (ensures (
+    let m' = List.Tot.fold_left (map_group_zero_or_more_match_item_serializer_op pkey pvalue m) accu l in
+    (cbor_map_mem kv m' <==> (match cbor_map_get accu (fst kv) with
+    | Some v_ -> v_ == snd kv
+    | None ->
+      let (k, v) = kv in
+      key k /\
+      value v /\
+      List.Tot.memP (pkey.parser k) l /\
+      begin match Map.get m (pkey.parser k) with
+      | None -> False
+      | Some v' ->
+        v == pvalue.serializer v'
+      end
+    ))
+  ))
+  (decreases l)
+= begin match l with
+    | [] -> ()
+    | a :: q ->
+      list_fold_map_group_zero_or_more_match_item_serializer_op_mem pkey pvalue m (map_group_zero_or_more_match_item_serializer_op pkey pvalue m accu a) q kv
+  end
+
+let rec list_fold_map_group_zero_or_more_match_item_serializer_length
+  (#tkey #tvalue: Type)
+  (#key #value: typ)
+  (pkey: spec key tkey true)
+  (#inj: bool)
+  (pvalue: spec value tvalue inj)
+  (m: Map.t pkey tvalue { Map.for_all (value_serializable pvalue) m })
+  (accu: cbor_map)
+  (l: list tkey)
+: Lemma
+  (requires (
+    List.Tot.no_repeats_p l /\
+    (forall x . List.Tot.memP x l ==> Map.defined x m) /\
+    (forall x . ~ (List.Tot.memP x l /\ cbor_map_defined (pkey.serializer x) accu))
+  ))
+  (ensures (
+    let m' = List.Tot.fold_left (map_group_zero_or_more_match_item_serializer_op pkey pvalue m) accu l in
+    cbor_map_length m' == cbor_map_length accu + List.Tot.length l
+  ))
+  (decreases l)
+= match l with
+  | [] -> ()
+  | a :: q ->
+    list_fold_map_group_zero_or_more_match_item_serializer_length pkey pvalue m (map_group_zero_or_more_match_item_serializer_op pkey pvalue m accu a) q
+
+let map_group_zero_or_more_match_item_serializer'
+  (#tkey #tvalue: Type)
+  (#key #value: typ)
+  (pkey: spec key tkey true)
+  (#inj: bool)
+  (pvalue: spec value tvalue inj)
+  (m: Map.t pkey tvalue { Map.for_all (value_serializable pvalue) m })
+: Tot cbor_map
+= Set.fold (map_group_zero_or_more_match_item_serializer_op pkey pvalue m) cbor_map_empty (Map.key_set m)
+
+let map_group_zero_or_more_match_item_serializer'_mem_aux
+  (#tkey #tvalue: Type)
+  (#key #value: typ)
+  (pkey: spec key tkey true)
+  (#inj: bool)
+  (pvalue: spec value tvalue inj)
+  (m: Map.t pkey tvalue { Map.for_all (value_serializable pvalue) m })
+  (kv: (cbor & cbor))
+: Tot prop
+=
+  let (k, v) = kv in
+      key k /\
+      value v /\
+      exists kv' . Map.mem kv' m /\
+      fst kv' == (pkey.parser k) /\
+      v == pvalue.serializer (snd kv')
+
+let map_group_zero_or_more_match_item_serializer'_mem
+  (#tkey #tvalue: Type)
+  (#key #value: typ)
+  (pkey: spec key tkey true)
+  (#inj: bool)
+  (pvalue: spec value tvalue inj)
+  (m: Map.t pkey tvalue { Map.for_all (value_serializable pvalue) m })
+  (kv: (cbor & cbor))
+: Lemma
+  (ensures (
+    let m' = map_group_zero_or_more_match_item_serializer' pkey pvalue m in
+    (cbor_map_mem kv m' <==> (map_group_zero_or_more_match_item_serializer'_mem_aux pkey pvalue m kv))
+  ))
+  [SMTPat (cbor_map_mem kv (map_group_zero_or_more_match_item_serializer' pkey pvalue m))]
+= let s = Map.key_set m in
+  let l = Set.set_as_list s in
+  Set.fold_eq (map_group_zero_or_more_match_item_serializer_op pkey pvalue m) cbor_map_empty s l;
+  list_fold_map_group_zero_or_more_match_item_serializer_op_mem pkey pvalue m cbor_map_empty l kv
+
+let map_group_zero_or_more_match_item_serializer'_length
+  (#tkey #tvalue: Type)
+  (#key #value: typ)
+  (pkey: spec key tkey true)
+  (#inj: bool)
+  (pvalue: spec value tvalue inj)
+  (m: Map.t pkey tvalue { Map.for_all (value_serializable pvalue) m })
+: Lemma
+  (ensures (
+    cbor_map_length (map_group_zero_or_more_match_item_serializer' pkey pvalue m) == Map.length m
+  ))
+  [SMTPat (cbor_map_length (map_group_zero_or_more_match_item_serializer' pkey pvalue m))]
+= let s = Map.key_set m in
+  let l = Set.set_as_list s in
+  Set.fold_eq (map_group_zero_or_more_match_item_serializer_op pkey pvalue m) cbor_map_empty s l;
+  list_fold_map_group_zero_or_more_match_item_serializer_length pkey pvalue m cbor_map_empty l
+
+#restart-solver
+let map_group_zero_or_more_match_item_serializer
+  (#tkey #tvalue: Type)
+  (#key #value: typ)
+  (pkey: spec key tkey true)
+  (#inj: bool)
+  (pvalue: spec value tvalue inj)
+: Tot (map_group_serializer_spec (map_group_zero_or_more_match_item_parser pkey pvalue))
 = fun x ->
-  map_group3_concat_unique_weak_zero_or_more_right source source;
-  let Some (l1, l2) = source x in
-  List.Tot.append_length l1 l2;
-  p l1 :: map_group_parser_spec_zero_or_more p target_size1 l2
+  let y = map_group_zero_or_more_match_item_serializer' pkey pvalue x in
+  assert (forall x . Some? (cbor_map_get y x) ==> cbor_map_mem (x, Some?.v (cbor_map_get y x)) y);
+  let py = map_group_zero_or_more_match_item_parser' pkey pvalue y in
+  assert (forall (kv: (tkey & tvalue)) . Map.mem kv x ==> cbor_map_mem (pkey.serializer (fst kv), pvalue.serializer (snd kv)) y);
+  assert (Map.equal' py x);
+  y
 
-let map_group_serializer_spec_one_or_more
-  (#source: nonempty_map_group)
-  (#target: Type)
-  (#target_size: target -> nat)
-  (#p: map_group_parser_spec source target_size)
-  (s: map_group_serializer_spec p {
-    map_group3_concat_unique_strong source source
-  })
-  (target_size1 : list target -> nat {
-    forall (l: list target) . target_size1 l == (if Nil? l then 0 else target_size (List.Tot.hd l) + target_size1 (List.Tot.tl l))
-  })
-  (target_size2 : nelist target -> nat {
-    forall (l: nelist target) . target_size2 l == target_size1 l
-  })
-: Tot (map_group_serializer_spec (map_group_parser_spec_one_or_more p target_size1 target_size2))
-= fun x ->
-  map_group3_concat_unique_weak_zero_or_more_right source source;
-  let hd :: tl = x in
-  let l1 = s hd in
-  let l2 = map_group_serializer_spec_zero_or_more s target_size1 tl in
-  List.Tot.append_length l1 l2;
-  l1 `List.Tot.append` l2
+let map_group_zero_or_more_match_item_parser_inj
+  (#tkey #tvalue: Type)
+  (#key #value: typ)
+  (pkey: spec key tkey true)
+  (#inj: bool)
+  (pvalue: spec value tvalue inj)
+  (m: cbor_map { map_group_serializer_spec_arg_prop (map_group_zero_or_more (map_group_match_item false key value)) key m })
+: Lemma
+  (requires inj)
+  (ensures (
+    map_group_zero_or_more_match_item_serializer pkey pvalue (map_group_zero_or_more_match_item_parser pkey pvalue m) `cbor_map_equal'` m
+  ))
+= let y = map_group_zero_or_more_match_item_parser pkey pvalue m in
+  let sy = map_group_zero_or_more_match_item_serializer pkey pvalue y in
+  assert (forall k . Some? (cbor_map_get m k) ==> cbor_map_mem (k, Some?.v (cbor_map_get m k)) m);
+  assert (forall k . Map.defined k y ==> Map.mem (k, Some?.v (Map.get y k)) y);
+  assert (cbor_map_filter (matches_map_group_entry key value) m `cbor_map_equal` m);
+  assert (forall (kv: (cbor & cbor)) . cbor_map_mem kv m ==> value (snd kv));
+  assert (forall (kv: (cbor & cbor)) . cbor_map_mem kv m ==> (value (snd kv) /\ Map.mem (pkey.parser (fst kv), pvalue.parser (snd kv)) y));
+  ()
 
-let map_group_parser_spec_zero_or_one
-  (#source: det_map_group)
-  (#target: Type)
-  (#target_size: target -> nat)
-  (p: map_group_parser_spec source target_size)
-  (target_size': option target -> nat {
-    forall x . target_size' x == begin match x with
-    | None -> 0
-    | Some x -> target_size x
-    end
-  })
-: Tot (map_group_parser_spec (map_group3_zero_or_one source) target_size')
-= fun x ->
-    if Some? (source x)
-    then Some (p x)
-    else None
-
-let map_group_serializer_spec_zero_or_one
-  (#source: nonempty_map_group) // needed because the empty case must map to None only
-  (#target: Type)
-  (#target_size: target -> nat)
-  (#p: map_group_parser_spec source target_size)
-  (s: map_group_serializer_spec p)
-  (target_size': option target -> nat {
-    forall x . target_size' x == begin match x with
-    | None -> 0
-    | Some x -> target_size x
-    end
-  })
-: Tot (map_group_serializer_spec (map_group_parser_spec_zero_or_one p target_size'))
-= fun x ->
-    match x with
-    | None -> []
-    | Some y -> s y
+let mg_zero_or_more_match_item
+  (#tkey #tvalue: Type)
+  (#key #value: typ)
+  (pkey: spec key tkey true)
+  (#inj: bool)
+  (pvalue: spec value tvalue inj)
+: Tot (mg_spec (map_group_zero_or_more (map_group_match_item false key value)) key (Map.t pkey tvalue) inj)
+= {
+  mg_size = map_group_zero_or_more_match_item_length pkey;
+  mg_serializable = Map.for_all (value_serializable pvalue);
+  mg_parser = map_group_zero_or_more_match_item_parser pkey pvalue;
+  mg_serializer = map_group_zero_or_more_match_item_serializer pkey pvalue;
+  mg_inj = Classical.forall_intro (Classical.move_requires (map_group_zero_or_more_match_item_parser_inj pkey pvalue));
+}
